<?xml version="1.0" ?>
<rdf:RDF 
	xml:base="http://www.example.it/myPMeffort#"

	xmlns:mpmo="http://robertocasadei.it/my-pm-ontology#"

	xmlns:rdf="http://www.w3.org/1999/02/22-rdf-syntax-ns#"
	xmlns:rdfs="http://www.w3.org/2000/01/rdf-schema#"

	xmlns:skos="http://www.w3.org/2004/02/skos/core#"
	xmlns:org="http://www.w3.org/ns/org#"
	xmlns:foaf="http://xmlns.com/foaf/0.1/"
	xmlns:time="http://www.w3.org/2006/time#"

	xmlns:doap="http://usefulinc.com/ns/doap#">

	<!-- **************************************************** -->
	<!-- ************************ CORE ********************** -->
	<!-- **************************************************** -->	

	<rdfs:Class rdf:about="http://robertocasadei.it/my-pm-ontology#PMModel"> 
		<!--is a PM concept?--> 
		<rdfs:subClassOf rdf:resource="http://www.w3.org/2004/02/skos/core#ConceptScheme" />
		<rdfs:label>Project management model</rdfs:label>
		<rdfs:comment>The class of all project management models, i.e., the class of those sets of concepts that can be used with the aim of successfully carrying out one or more project management efforts.</rdfs:comment>
	</rdfs:Class>
	<rdfs:Class rdf:about="http://robertocasadei.it/my-pm-ontology#PMConcept"> 
		<!--is a PM concept itself?-->
		<rdfs:subClassOf rdf:resource="http://www.w3.org/2004/02/skos/core#Concept" />
		<rdfs:label>Project management concept</rdfs:label>
		<rdfs:comment>The class of all project management concepts, i.e., the class of the concepts that can be used within a project management model.</rdfs:comment>
	</rdfs:Class>
	<rdfs:Class rdf:about="http://robertocasadei.it/my-pm-ontology#PMEffort"> 
		<!--is a PM concept?-->
		<rdfs:label>Project management effort</rdfs:label>
		<rdfs:comment>The class of all project management efforts, i.e., the class of the endeavours which should be governed using project management techniques.</rdfs:comment>
	</rdfs:Class>

	<!-- **************************************************** -->
	<!-- ******************** PM CONCEPTS ******************* -->
	<!-- **************************************************** -->

	<rdfs:Class rdf:about="http://robertocasadei.it/my-pm-ontology#Process">
		<rdfs:type rdf:resource="http://robertocasadei.it/my-pm-ontology#PMConcept" />
		<rdfs:subClassOf rdf:resource="http://robertocasadei.it/my-pm-ontology#PMEffort" />
		<rdfs:label>Process</rdfs:label>
		<rdfs:comment>A process is a set of interrelated actions and activities performed to create a pre-specified product, service, or result. Each process is characterized by its inputs, the tools and techniques that can be applied, and the resulting outputs.</rdfs:comment>
	</rdfs:Class>
	<rdfs:Class rdf:about="http://robertocasadei.it/my-pm-ontology#Project">
		<rdfs:subClassOf rdf:resource="http://robertocasadei.it/my-pm-ontology#Process" />
		<rdfs:label>Project</rdfs:label>
		<rdfs:comment>A project is temporary endeavor undertaken to create a unique product, service, or result.</rdfs:comment>
	</rdfs:Class>
	<rdfs:Class rdf:about="http://robertocasadei.it/my-pm-ontology#Organization">
		<rdfs:type rdf:resource="http://robertocasadei.it/my-pm-ontology#PMConcept" />
		<rdfs:subClassOf rdf:resource="http://www.w3.org/ns/org#Organization" />
		<rdfs:label>Organization</rdfs:label>
		<rdfs:comment>An organization is a group of individuals organized to work for some purpose or mission.</rdfs:comment>
	</rdfs:Class>
	<rdfs:Class rdf:about="http://robertocasadei.it/my-pm-ontology#ValueResource">
		<rdfs:type rdf:resource="http://robertocasadei.it/my-pm-ontology#PMConcept" />
		<rdfs:label>Value resource</rdfs:label>
		<rdfs:comment>Anything expected to produce value through interaction with other entities.</rdfs:comment>
	</rdfs:Class>	
	<rdfs:Class rdf:about="http://robertocasadei.it/my-pm-ontology#Deliverable">
		<rdfs:subClassOf rdf:resource="http://robertocasadei.it/my-pm-ontology#ValueResource" />
		<rdfs:label>Deliverable</rdfs:label>
		<rdfs:comment>A deliverable is any unique and verifiable product, result or capability to perform a service that is required to be produced to complete a process, phase, or project.</rdfs:comment>
	</rdfs:Class>
	<rdfs:Class rdf:about="http://robertocasadei.it/my-pm-ontology#Participant">
		<rdfs:type rdf:resource="http://robertocasadei.it/my-pm-ontology#PMConcept" />
		<rdfs:subClassOf rdf:resource="http://xmlns.com/foaf/0.1/Agent" />
		<rdfs:label>Participant</rdfs:label>
		<rdfs:comment>An agent (which may be a person but not necessarily) which actively does something within a project.</rdfs:comment>
	</rdfs:Class>
	<rdfs:Class rdf:about="http://robertocasadei.it/my-pm-ontology#Role">
		<rdfs:type rdf:resource="http://robertocasadei.it/my-pm-ontology#PMConcept" />
		<rdfs:subClassOf rdf:resource="http://www.w3.org/ns/org#Role" />
		<rdfs:label>Role</rdfs:label>
		<rdfs:comment>A role within a project.</rdfs:comment>
	</rdfs:Class> 
	<rdfs:Class rdf:about="http://robertocasadei.it/my-pm-ontology#Stakeholder">
		<rdfs:type rdf:resource="http://robertocasadei.it/my-pm-ontology#PMConcept" />
		<rdfs:subClassOf rdf:resource="http://xmlns.com/foaf/0.1/Person" />
		<rdfs:label>Stakeholder</rdfs:label>
		<rdfs:comment>A project stakeholder, i.e., a person which has an interest in the project.</rdfs:comment>		
	</rdfs:Class>
	<rdfs:Class rdf:about="http://robertocasadei.it/my-pm-ontology#Membership">
		<rdfs:type rdf:resource="http://robertocasadei.it/my-pm-ontology#PMConcept" />
		<rdfs:subClassOf rdf:resource="http://www.w3.org/ns/org#Membership" />
		<rdfs:label>Membership</rdfs:label>
		<rdfs:comment>A membership relationship (agent, role, organization, project/process) within a project.</rdfs:comment>		
	</rdfs:Class>

	<!-- **************************************************** -->
	<!-- ****************** SPECIALIZATIONS ***************** -->
	<!-- **************************************************** -->
	<rdfs:Class rdf:about="http://robertocasadei.it/my-pm-ontology#SoftwareProject">
		<rdfs:subClassOf rdf:resource="http://robertocasadei.it/my-pm-ontology#Project" />
		<rdfs:subClassOf rdf:resource="http://usefulinc.com/ns/doap#Project" />
		<rdfs:label>Software project</rdfs:label>
		<rdfs:comment>A software project, i.e., a project which deals with the construction and delivery of software-based results.</rdfs:comment>
	</rdfs:Class>

	<!-- **************************************************** -->
	<!-- ****************** RDFS PROPERTIES ***************** -->
	<!-- **************************************************** -->
	<rdfs:Property rdf:about="http://robertocasadei.it/my-pm-ontology#governsExecutionOf">
		<rdfs:domain rdf:resource="http://robertocasadei.it/my-pm-ontology#PMModel" />
		<rdfs:range rdf:resource="http://robertocasadei.it/my-pm-ontology#Project" />
		<rdfs:comment>It states that the given project management model (subject) is applied to the given project (object)</rdfs:comment>
	</rdfs:Property>
	<rdfs:Property rdf:about="http://robertocasadei.it/my-pm-ontology#hasInput">
		<rdfs:domain rdf:resource="http://robertocasadei.it/my-pm-ontology#PMConcept" />
		<rdfs:range rdf:resource="http://robertocasadei.it/my-pm-ontology#PMConcept" />
		<rdfs:comment>It states that the given project management concept (subject) has the given project management concept (object) as input</rdfs:comment>		
	</rdfs:Property>
	<rdfs:Property rdf:about="http://robertocasadei.it/my-pm-ontology#hasOutput">
		<rdfs:domain rdf:resource="http://robertocasadei.it/my-pm-ontology#PMConcept" />
		<rdfs:range rdf:resource="http://robertocasadei.it/my-pm-ontology#PMConcept" />
		<rdfs:comment>It states that the given project management concept (subject) has the given project management concept (object) as output</rdfs:comment>		
	</rdfs:Property>
	<rdfs:Property rdf:about="http://robertocasadei.it/my-pm-ontology#withinProcess">
		<rdfs:domain rdf:resource="http://robertocasadei.it/my-pm-ontology#Membership" />
		<rdfs:range rdf:resource="http://robertocasadei.it/my-pm-ontology#Process" />
		<rdfs:comment>It states that the given membership (subject) applies within the given process (object).</rdfs:comment>		
	</rdfs:Property>

	<!-- **************************************************** -->
	<!-- ********************* INSTANCES ******************** -->
	<!-- **************************************************** -->

	<mpmo:PMModel rdf:about="http://robertocasadei.it/my-pm-ontology#SimplePMM">
		<rdfs:subClassOf rdf:resource="http://robertocasadei.it/my-pm-ontology#PMModel" />
		<skos:hasTopConcept rdf:resource="http://robertocasadei.it/my-pm-ontology#Organization" />
		<skos:hasTopConcept rdf:resource="http://robertocasadei.it/my-pm-ontology#Process" />			
		<skos:hasTopConcept rdf:resource="http://robertocasadei.it/my-pm-ontology#Project" />
		<skos:hasTopConcept rdf:resource="http://robertocasadei.it/my-pm-ontology#ValueResource" />		
		<skos:hasTopConcept rdf:resource="http://robertocasadei.it/my-pm-ontology#Deliverable" />
		<skos:hasTopConcept rdf:resource="http://robertocasadei.it/my-pm-ontology#Participant" />
		<skos:hasTopConcept rdf:resource="http://robertocasadei.it/my-pm-ontology#Stakeholder" />				
		<skos:hasTopConcept rdf:resource="http://robertocasadei.it/my-pm-ontology#Role" />		
		<skos:hasTopConcept rdf:resource="http://robertocasadei.it/my-pm-ontology#Membership" />		
	</mpmo:PMModel>

	<mpmo:Role rdf:about="http://robertocasadei.it/my-pm-ontology#Customer">
		<rdfs:label>Customer</rdfs:label>
		<rdfs:comment>A customer is the recipient of a good, service, product, or idea, obtained from a seller, vendor, or supplier for a monetary or other valuable consideration.</rdfs:comment>
	</mpmo:Role>		

	<!-- AN EXAMPLE: "THIS ASSIGNMENT" DESCRIBED IN THE CONTEXT OF THE ONTOLOGY -->
	<mpmo:SoftwareProject rdf:ID="ThisAssignment">
		<mpmo:hasInput rdf:resource="#PMModelForThisAssignment" /> 			<!-- PM Model -->
		<mpmo:hasInput rdf:resource="#MyOrganization" /> 					<!-- Organization -->			
		<mpmo:hasInput rdf:resource="#RobertoCasadei" /> 					<!-- Participant -->
		<mpmo:hasInput rdf:resource="#AntonellaCarbonaro" /> 				<!-- Stakeholder -->		
		<mpmo:hasInput rdf:resource="#Factotum" /> 							<!-- Role 1 -->
		<mpmo:hasInput rdf:resource="#Customer" /> 							<!-- Role 2 -->

		<mpmo:hasOutput rdf:resource="#ThisRDFSFile" /> 					<!-- Deliverable -->
		<mpmo:hasOutput rdf:resource="#PresentationForThisAssignment" /> 	<!-- Deliverable -->

		<doap:created>2014-04-10</doap:created>
		<doap:maintainer rdf:resource="#RobertoCasadei" />
	</mpmo:SoftwareProject>
	<mpmo:SimplePMM rdf:ID="PMModelForThisAssignment">
		<mpmo:governsExecutionOf rdf:resource="#ThisAssignment" />
	</mpmo:SimplePMM>
	<mpmo:Organization rdf:ID="MyOrganization">
		<rdfs:comment>My organization (composed only by me).</rdfs:comment>
	</mpmo:Organization>
	<mpmo:Organization rdf:ID="Unibo">
		<rdfs:label>Alma Mater Studiorum - Universit√† di Bologna</rdfs:label>
	</mpmo:Organization>
	<mpmo:Participant rdf:ID="RobertoCasadei">
	   <foaf:name>Roberto Casadei</foaf:name>
	   <foaf:title>Dr.</foaf:title>
	   <foaf:firstName>Roberto</foaf:firstName>
	   <foaf:surname>Casadei</foaf:surname>
	   <foaf:nick>robyonrails</foaf:nick>
	   <foaf:mbox>mailto:roberto.casadei12@studio.unibo.it</foaf:mbox>
	</mpmo:Participant>
	<mpmo:Stakeholder rdf:ID="AntonellaCarbonaro">
		<foaf:name>Antonella Carbonaro</foaf:name>
		<foaf:firstName>Antonella</foaf:firstName>
		<foaf:surname>Carbonaro</foaf:surname>
		<foaf:mbox>mailto:antonella.carbonaro@unibo.it</foaf:mbox>
	</mpmo:Stakeholder>
	<mpmo:Membership rdf:ID="MyEngagement">
		<org:organization rdf:resource="#MyOrganization" />
		<org:member rdf:resource="#RobertoCasadei" />
		<mpmo:withinProcess rdf:resource="#ThisAssignment" />
		<org:role>
			<mpmo:Role rdf:ID="Factotum">
				<rdfs:comment>The person who does everything.</rdfs:comment>
			</mpmo:Role>
		</org:role>
		<org:memberDuring>
			<time:Interval>
				<time:inside>
					<time:inDateTime><time:April /></time:inDateTime>
				</time:inside>
			</time:Interval>
		</org:memberDuring>
	</mpmo:Membership>
	<mpmo:Membership rdf:ID="ProfEngagement">
		<org:organization rdf:resource="#Unibo" />
		<org:member rdf:resource="#AntonellaCarbonaro" />
		<mpmo:withinProcess rdf:resource="#ThisAssignment" />
		<org:role rdf:resource="http://robertocasadei.it/my-pm-ontology#Customer" />
	</mpmo:Membership>
	<mpmo:Deliverable rdf:ID="ThisRDFSFile" />
	<mpmo:Deliverable rdf:ID="PresentationForThisAssignment" />

</rdf:RDF>